end of day 28/12/18

michael_formal/Contexts.thy
@@ -227,10 +227,16 @@ primrec posterior_sequence :: "context \<Rightarrow> transition_matrix \<Rightar
       _ \<Rightarrow> c
     )"
 
+definition datastate2context :: "datastate \<Rightarrow> context" where
+  "datastate2context d = (\<lambda>x. case x of V r \<Rightarrow> (case d r of None \<Rightarrow> Undef | Some v \<Rightarrow> Eq v) | _ \<Rightarrow> \<lbrakk>\<rbrakk> x)"
+
+definition satisfies_context :: "datastate \<Rightarrow> context \<Rightarrow> bool" where
+  "satisfies_context d c = consistent (conjoin (datastate2context d) c)"
+
 (* Does t2 subsume t1? *)
 definition subsumes :: "context \<Rightarrow> transition \<Rightarrow> transition \<Rightarrow> bool" where (* Corresponds to Algorithm 2 in Foster et. al. *)
   "subsumes c t2 t1 \<equiv> (\<forall>r i. (cval (medial c (Guard t1) r) i = Some True) \<longrightarrow> (cval (medial c (Guard t2) r) i) = Some True) \<and>
-                      (\<forall> i r. apply_guards (Guard t1) (join_ir i r) \<longrightarrow> apply_outputs (Outputs t1) (join_ir i r) = apply_outputs (Outputs t2) (join_ir i r)) \<and>
+                      (\<forall> i r. satisfies_context r c \<longrightarrow> apply_guards (Guard t1) (join_ir i r) \<longrightarrow> apply_outputs (Outputs t1) (join_ir i r) = apply_outputs (Outputs t2) (join_ir i r)) \<and>
                       (\<forall>r i. cval (posterior (medial c (Guard t1)) t2 r) i = Some True \<longrightarrow> (cval (posterior c t1 r) i = Some True) \<or> (posterior c t1 r) = Undef) \<and>
                       (consistent (posterior c t1) \<longrightarrow> consistent (posterior c t2))"
 
@@ -239,8 +245,8 @@ definition anterior_context :: "transition_matrix \<Rightarrow> trace \<Rightarr
 
 (* Does t1 subsume t2 in all possible anterior contexts? *)
 (* For every path which gets us to the problem state, does t1 subsume t2 in the resulting context *)
-definition directly_subsumes :: "transition_matrix \<Rightarrow> nat \<Rightarrow> transition \<Rightarrow> transition \<Rightarrow> bool" where
-  "directly_subsumes e s t1 t2 = (\<forall>p. (gets_us_to s e 0 <>  p) \<longrightarrow> subsumes (anterior_context e p) t1 t2)"
+definition directly_subsumes :: "transition_matrix \<Rightarrow> transition_matrix \<Rightarrow> nat \<Rightarrow> transition \<Rightarrow> transition \<Rightarrow> bool" where
+  "directly_subsumes e1 e2 s t1 t2 = (\<forall>p. accepts_trace e1 p \<longrightarrow> (gets_us_to s e1 0 <>  p) \<longrightarrow> subsumes (anterior_context e2 p) t1 t2)"
 
 primrec pairs2guard :: "(aexp \<times> cexp) list \<Rightarrow> guard" where
   "pairs2guard [] = gexp.Bc True" |
