michael_formal/Nondeterministic_EFSM.thy
@@ -20,16 +20,35 @@ primrec nondeterministic_observe_all :: "transition_matrix \<Rightarrow> nat \<R
 definition nondeterministic_observe_trace :: "transition_matrix \<Rightarrow> nat \<Rightarrow> datastate \<Rightarrow> trace \<Rightarrow> observation" where
   "nondeterministic_observe_trace e s r t \<equiv> map (\<lambda>(t,x,y,z). y) (nondeterministic_observe_all e s r t)"
 
-inductive nondeterministic_simulates_trace :: "transition_matrix \<Rightarrow> transition_matrix \<Rightarrow> nat \<Rightarrow> nat \<Rightarrow> datastate \<Rightarrow> datastate \<Rightarrow> trace \<Rightarrow> bool" where
-  base: "nondeterministic_simulates_trace e1 e2 s1 s2 d1 d2 []" |
-  step_some: "nondeterministic_step e1 s1 d1 l i = Some (tr1, s1', p', d1') \<Longrightarrow>
+inductive nondeterministic_simulates_trace :: "transition_matrix \<Rightarrow> transition_matrix \<Rightarrow> nat \<Rightarrow> nat \<Rightarrow> datastate \<Rightarrow> datastate \<Rightarrow> trace \<Rightarrow> (nat \<Rightarrow> nat) \<Rightarrow> bool" where
+  base: "nondeterministic_simulates_trace e2 e1 s2 s1 d2 d1 [] _" |
+  step_some: "s2 = H s1 \<Longrightarrow>
+              nondeterministic_step e1 s1 d1 l i = Some (tr1, s1', p', d1') \<Longrightarrow>
               (s2', tr2) |\<in>| possible_steps e2 s2 d2 l i \<Longrightarrow>
               d2' = (apply_updates (Updates tr2) (join_ir i d2) d2) \<Longrightarrow>
-              nondeterministic_simulates_trace e1 e2 s1' s2' d1' d2' t \<Longrightarrow>
-              nondeterministic_simulates_trace e1 e2 s1 s2 d1 d2 ((l, i)#t)" |
-  step_none: "nondeterministic_step e1 s1 d1 l i = None \<Longrightarrow> nondeterministic_simulates_trace e1 e2 s1 s2 d1 d2 ((l, i)#t)"
+              nondeterministic_simulates_trace e2 e1 s2' s1' d2' d1' t H \<Longrightarrow>
+              nondeterministic_simulates_trace e2 e1 s2 s1 d2 d1 ((l, i)#t) H" |
+  step_none: "nondeterministic_step e1 s1 d1 l i = None \<Longrightarrow> nondeterministic_simulates_trace e2 e1 s2 s1 d2 d1 ((l, i)#t) _"
 
-definition nondeterministic_simulates :: "transition_matrix \<Rightarrow> transition_matrix \<Rightarrow> bool" where
-  "nondeterministic_simulates m1 m2 = (\<forall>t. nondeterministic_simulates_trace m1 m2 0 0 <> <> t)"
+lemma nondeterministic_step_none: "nondeterministic_step e s r l i = None \<Longrightarrow> step e s r l i = None"
+proof-
+  assume premise: "nondeterministic_step e s r l i = None"
+  have aux1: "\<forall>a b. (a, b) |\<notin>| possible_steps e s r l i \<Longrightarrow>
+        possible_steps e s r l i = {||}"
+    by auto
+  show ?thesis
+    using premise
+    apply (simp add: step_def nondeterministic_step_def)
+    apply (case_tac "\<exists>a b. (a, b) |\<in>| possible_steps e s r l i")
+     apply simp
+     apply (cases "SOME x. x |\<in>| possible_steps e s r l i")
+     apply simp
+    apply simp
+    apply clarify
+    by (simp add: aux1)
+qed
+
+definition nondeterministic_simulates :: "transition_matrix \<Rightarrow> transition_matrix \<Rightarrow> (nat \<Rightarrow> nat) \<Rightarrow> bool" where
+  "nondeterministic_simulates m2 m1 H = (\<forall>t. nondeterministic_simulates_trace m2 m1 0 0 <> <> t H)"
 
 end
