michael_formal/not4afp/Paper_Example.thy
@@ -29,6 +29,9 @@ definition coin :: transition where
               Updates = [(R 2, Plus (V (R 2)) (V (I 1)))]
             \<rparr>"
 
+lemma guard_coin: "Guard coin = []"
+  by (simp add: coin_def)
+
 definition vend_fail :: transition where
   "vend_fail = \<lparr>
               Label = ''vend'',
@@ -68,6 +71,20 @@ proof-
     by (simp add: transitions remove_input_constraints_def)
 qed
 
+lemma select_posterior: "posterior \<lbrakk>\<rbrakk> select = \<lbrakk>V (R 1) \<mapsto> Bc True\<rbrakk>"
+  unfolding posterior_def Let_def
+  apply (rule ext)
+  by (simp add: transitions remove_input_constraints_def)
+
+lemma coin50_posterior: "posterior \<lbrakk>V (R 1) \<mapsto> cexp.Bc True\<rbrakk> coin50 = \<lbrakk>V (R 1) \<mapsto> cexp.Bc True, V (R 2) \<mapsto> Eq (Num 50)\<rbrakk>"
+  unfolding posterior_def Let_def
+  apply (rule ext)
+  apply (simp add: transitions remove_input_constraints_def)
+  apply (simp add: consistent_def)
+  apply (rule_tac x="<I 1 := Num 50>" in exI)
+  apply clarify
+  by (simp add: consistent_empty_4)
+
 definition drinks_before :: transition_matrix where
   "drinks_before = {|((0, 1), select), ((1, 2), coin50), ((2, 2), coin), ((2, 2), vend_fail), ((2, 3), vend_success)|}"
 
@@ -83,8 +100,8 @@ lemma merge_1_2: "merge_states 1 2 drinks_before = merge_1_2"
 definition merge_1_2_update :: transition_matrix where
   "merge_1_2_update = {|((0, 1), select_update), ((1, 1), coin50), ((1, 1), coin), ((1, 1), vend_fail), ((1, 3), vend_success)|}"
 
-definition mapping :: "nat \<Rightarrow> nat" where
-  "mapping x = (if x = 0 then 0 else if x = 1 then 1 else if x = 2 then 1 else x)"
+definition update_mapping :: "nat \<Rightarrow> nat" where
+  "update_mapping x = x"
 
 lemma possible_steps_drinks_before_select: "length b = 1 \<Longrightarrow> possible_steps drinks_before 0 r ''select'' b = {|(1, select)|}"
 proof-
@@ -388,7 +405,10 @@ proof-
     by (simp add: nondeterministic_step_def possible_steps_def ffilter_def set_filter)
 qed
 
-lemma simulation_2_1: "\<forall>r. nondeterministic_simulates_trace drinks_before merge_1_2_update 2 1 r r lst"
+definition update_before :: "nat \<Rightarrow> nat" where
+  "update_before x = (if x = 2 then 1 else x)"
+
+lemma simulation_2_1: "\<forall>r. nondeterministic_simulates_trace merge_1_2_update drinks_before 1 2 r r lst update_before"
 proof (induct lst)
   case Nil
   then show ?case
@@ -402,6 +422,7 @@ next
     apply (case_tac "aa = ''coin'' \<and> length b = 1")
      apply simp
      apply (rule nondeterministic_simulates_trace.step_some)
+         apply (simp add: update_before_def)
         apply (simp add: nondeterministic_step_def possible_steps_drinks_before_coin)
     using possible_steps_merge_1_2_update_coin
        apply blast
@@ -424,11 +445,13 @@ next
     apply simp
     apply (case_tac "x1 < 100")
      apply (rule nondeterministic_simulates_trace.step_some)
+         apply (simp add: update_before_def)
         apply (simp add: nondeterministic_step_def drinks_before_vend_fail)
        apply (simp add: merge_1_2_update_vend_fail)
       apply simp
      apply (simp add: vend_fail_def)
-     apply (rule nondeterministic_simulates_trace.step_some)
+    apply (rule nondeterministic_simulates_trace.step_some)
+        apply (simp add: update_before_def)
        apply (simp add: nondeterministic_step_def drinks_before_vend_success)
       apply (simp add: merge_1_2_update_vend_success)
      apply simp
@@ -441,7 +464,7 @@ next
     by (simp add: drinks_before_ends_at_3)
   qed
 
-lemma simulation_1_1: "nondeterministic_simulates_trace drinks_before merge_1_2_update 1 1 <R 1 := d> <R 1 := d, R 2 := Num 0> ((aa, b) # list)"
+lemma simulation_1_1: "nondeterministic_simulates_trace merge_1_2_update drinks_before 1 1 <R 1 := d, R 2 := Num 0> <R 1 := d> ((aa, b) # list) update_before"
 proof-
   have choice_coin50_coin: "(\<exists>a b. a = 1 \<and> b = coin50 \<or> a = 1 \<and> b = coin)"
     by auto
@@ -469,9 +492,9 @@ proof-
      apply (rule nondeterministic_simulates_trace.step_none)
     using drinks_before_1_invalid
     apply auto[1]
-    
     apply (rule nondeterministic_simulates_trace.step_some)
-     apply (simp add: nondeterministic_step_def possible_steps_drinks_before_coin_50)
+        apply (simp add: update_before_def)
+       apply (simp add: nondeterministic_step_def possible_steps_drinks_before_coin_50)
       apply (simp add: nondeterministic_step_def merge_1_2_update_possible_steps_coin_50 choice_coin50_coin)
       apply auto[1]
      apply simp
@@ -479,7 +502,7 @@ proof-
     by (simp add: simulation_2_1)
 qed
 
-lemma simulation_0_0: "nondeterministic_simulates_trace drinks_before merge_1_2_update 0 0 Map.empty Map.empty ((aa, b) # t)"
+lemma simulation_0_0: "nondeterministic_simulates_trace merge_1_2_update drinks_before 0 0 Map.empty Map.empty ((aa, b) # t) update_before"
 proof-
   have select_updates: "length b = 1 \<Longrightarrow> (EFSM.apply_updates (Updates select) (case_vname (\<lambda>n. input2state b 1 (I n)) Map.empty) Map.empty) = <R 1 := hd b>"
     apply (rule ext)
@@ -490,12 +513,13 @@ proof-
     by (simp add: hd_input2state)
   show ?thesis
   apply (case_tac "aa = ''select'' \<and> length b = 1")
-   apply (rule nondeterministic_simulates_trace.step_some)
-     apply (simp add: nondeterministic_step_def possible_steps_drinks_before_select)
+     apply (rule nondeterministic_simulates_trace.step_some)
+         apply (simp add: update_before_def)
+        apply (simp add: nondeterministic_step_def possible_steps_drinks_before_select)
        apply (simp add: nondeterministic_step_def possible_steps_merge_1_2_update_select transitions)
-    apply simp
-   defer
-   apply (rule nondeterministic_simulates_trace.step_none)
+      apply simp
+     defer
+     apply (rule nondeterministic_simulates_trace.step_none)
      apply (simp add: drinks_before_step_0_invalid)
     apply (simp add: select_updates select_update_updates)
     apply (case_tac t)
@@ -504,7 +528,7 @@ proof-
     by (simp add: simulation_1_1)
 qed
 
-lemma simulation_aux: "nondeterministic_simulates_trace drinks_before merge_1_2_update 0 0 Map.empty Map.empty t"
+lemma simulation_aux: "nondeterministic_simulates_trace merge_1_2_update drinks_before 0 0 Map.empty Map.empty t update_before"
 proof (induct t)
 case Nil
   then show ?case
@@ -517,7 +541,7 @@ next
     by (simp add: simulation_0_0)
 qed
 
-lemma simulation: "nondeterministic_simulates drinks_before merge_1_2_update"
+lemma simulation: "nondeterministic_simulates merge_1_2_update drinks_before update_before"
   apply (simp add:nondeterministic_simulates_def)
   apply (rule allI)
   by (simp add: simulation_aux)
@@ -644,136 +668,227 @@ lemma select_first: "\<not> (aa = ''select'' \<and> length b = 1) \<Longrightarr
 
 lemma no_subsumption_empty: "\<not> subsumes \<lbrakk>\<rbrakk> coin coin50"
 proof-
-  have violation: "(\<exists>i r. apply_guards (Guard coin50) (case_vname (\<lambda>n. input2state i 1 (I n)) (\<lambda>n. r (R n))) \<and>
+  have violation: "(\<exists>i r. satisfies_context r \<lbrakk>\<rbrakk> \<and>
+           apply_guards (Guard coin50) (case_vname (\<lambda>n. input2state i 1 (I n)) (\<lambda>n. r (R n))) \<and>
            apply_outputs (Outputs coin50) (case_vname (\<lambda>n. input2state i 1 (I n)) (\<lambda>n. r (R n))) \<noteq>
            apply_outputs (Outputs coin) (case_vname (\<lambda>n. input2state i 1 (I n)) (\<lambda>n. r (R n))))"
     apply (rule_tac x="[Num 50]" in exI)
     apply (rule_tac x="<>" in exI)
-    by (simp add: transitions)
+    apply (simp add: transitions)
+    apply (simp add: satisfies_context_def datastate2context_def consistent_def)
+    apply (rule_tac x="<>" in exI)
+    apply safe
+    apply (case_tac r)
+       apply simp
+      apply simp
+      apply (case_tac x2)
+       apply simp
+      apply simp
+     apply simp
+    by simp
   show ?thesis
     by (simp add: subsumes_def violation)
 qed
 
-lemma "gets_us_to 1 merge_1_2_update 0 Map.empty p \<longrightarrow> subsumes (anterior_context merge_1_2_update p) coin coin50"
-proof(induct p)
-  case Nil
-  have "\<not>gets_us_to 1 merge_1_2_update 0 Map.empty []"
-    apply safe
-    apply (rule gets_us_to.cases)
-    by auto
-  then show ?case
+lemma satisfies_must_have_r2_0: "satisfies_context d \<lbrakk>V (R 1) \<mapsto> cexp.Bc True, V (R 2) \<mapsto> cexp.Eq (Num 0)\<rbrakk> \<Longrightarrow> d (R 2) = Some (Num 0)"
+proof-
+  have contrapositive: "\<not> d (R 2) = Some (Num 0) \<Longrightarrow> \<not>satisfies_context d \<lbrakk>V (R 1) \<mapsto> cexp.Bc True, V (R 2) \<mapsto> cexp.Eq (Num 0)\<rbrakk>"
+    apply (simp add: satisfies_context_def datastate2context_def consistent_def)
+    apply (rule allI)
+    apply (rule_tac x="V (R 2)" in exI)
+    apply simp
+    apply (case_tac "d (R 2)")
+     apply simp
     by simp
-next
-  case (Cons a p)
-    then show ?case
-    proof-
-      have select_updates: "\<forall>b. length b = 1 \<longrightarrow> (EFSM.apply_updates (Updates select_update) (case_vname (\<lambda>n. input2state b 1 (I n)) Map.empty) Map.empty) = <R 1 := hd b, R 2 := Num 0>"
-        apply clarify
-        apply (rule ext)
-        apply (simp add: transitions)
-        by (simp add: hd_input2state)
-      show ?thesis
-        apply (case_tac a)
-        apply clarify
-        apply (case_tac "aa = ''select'' \<and> length b = 1")
-         defer
-         apply (simp add: select_first)
-        apply (simp add: anterior_context_def step_def)
-        apply (simp add: possible_steps_merge_1_2_update_select select_update_posterior select_updates)
-        apply (case_tac p)
-        apply simp
-    qed
+  show "satisfies_context d \<lbrakk>V (R 1) \<mapsto> cexp.Bc True, V (R 2) \<mapsto> cexp.Eq (Num 0)\<rbrakk> \<Longrightarrow> d (R 2) = Some (Num 0)"
+    using contrapositive
+    by auto
+qed 
+
+lemma consistent_medial_coin: "consistent \<lbrakk>V (R 1) \<mapsto> cexp.Bc True, V (R 2) \<mapsto> cexp.Eq (Num 0)\<rbrakk>"
+    apply (simp add: consistent_def)
+    apply (rule_tac x="<R 1 := Str ''coke'', R 2 := Num 0, I 1 := Num 50>" in exI)
+    apply (rule allI)
+    by (simp add: consistent_empty_4)
+
+lemma coin_posterior: "posterior \<lbrakk>V (R 1) \<mapsto> cexp.Bc True, V (R 2) \<mapsto> cexp.Eq (Num 0)\<rbrakk> coin = 
+                       \<lbrakk>V (R 1) \<mapsto> cexp.Bc True, V (R 2) \<mapsto> cexp.Bc True\<rbrakk>"
+  apply (simp add: posterior_def Let_def transitions satisfiable_def remove_input_constraints_def)
+  apply standard
+  apply clarify
+   apply (rule ext)
+   apply simp
+  by (simp add: consistent_medial_coin)
+
+lemma coin_subsumes_coin50: "subsumes \<lbrakk>V (R 1) \<mapsto> cexp.Bc True, V (R 2) \<mapsto> cexp.Eq (Num 0)\<rbrakk> coin coin50"
+proof-
+  have medial_coin50: "medial \<lbrakk>V (R 1) \<mapsto> cexp.Bc True, V (R 2) \<mapsto> cexp.Eq (Num 0)\<rbrakk> (Guard coin50) =
+        \<lbrakk>V (R 1) \<mapsto> cexp.Bc True, V (R 2) \<mapsto> cexp.Eq (Num 0), V (I 1) \<mapsto> Eq (Num 50)\<rbrakk>"
+    apply (rule ext)
+    by (simp add: transitions)
+  have consistent_medial_coin50: "consistent \<lbrakk>V (R 1) \<mapsto> cexp.Bc True, V (R 2) \<mapsto> cexp.Eq (Num 0), V (I 1) \<mapsto> cexp.Eq (Num 50)\<rbrakk>"
+    apply (simp add: consistent_def)
+    apply (rule_tac x="<R 1 := Str ''coke'', R 2 := Num 0, I 1 := Num 50>" in exI)
+    apply (rule allI)
+    by (simp add: consistent_empty_4)
+  have apply_coin50_updates: "(remove_input_constraints
+              (Contexts.apply_updates \<lbrakk>V (R 1) \<mapsto> cexp.Bc True, V (R 2) \<mapsto> cexp.Eq (Num 0), V (I 1) \<mapsto> cexp.Eq (Num 50)\<rbrakk>
+                \<lbrakk>V (R 1) \<mapsto> cexp.Bc True, V (R 2) \<mapsto> cexp.Eq (Num 0)\<rbrakk> (Updates coin50))) = \<lbrakk>V (R 1) \<mapsto> cexp.Bc True, V (R 2) \<mapsto> cexp.Eq (Num 50)\<rbrakk>"
+    apply (rule ext)
+    by (simp add: coin50_def remove_input_constraints_def)
+  have apply_coin_updates: "remove_input_constraints
+                  (Contexts.apply_updates \<lbrakk>V (R 1) \<mapsto> cexp.Bc True, V (R 2) \<mapsto> cexp.Eq (Num 0), V (I 1) \<mapsto> cexp.Eq (Num 50)\<rbrakk>
+                    \<lbrakk>V (R 1) \<mapsto> cexp.Bc True, V (R 2) \<mapsto> cexp.Eq (Num 0), V (I 1) \<mapsto> cexp.Eq (Num 50)\<rbrakk> (Updates coin)) = \<lbrakk>V (R 1) \<mapsto> cexp.Bc True, V (R 2) \<mapsto> cexp.Eq (Num 50)\<rbrakk>"
+    apply (rule ext)
+    apply (simp add: coin_def remove_input_constraints_def valid_def satisfiable_def)
+    by auto
+  show ?thesis
+    unfolding subsumes_def
+    apply standard
+     apply (simp add: transitions)
+     apply clarify
+     apply (case_tac "cval (\<lbrakk>\<rbrakk> r) i")
+      apply simp
+     apply simp
+    apply standard
+     apply (simp add: transitions)
+     apply clarify
+     apply (case_tac "value_plus (r (R 2)) (Some (Num 50))")
+      apply simp
+    using satisfies_must_have_r2_0
+      apply fastforce
+     apply simp
+    using satisfies_must_have_r2_0
+     apply fastforce
+    apply standard
+     apply (simp add: medial_coin50)
+     apply clarify
+     apply (simp add: posterior_def Let_def guard_coin medial_coin50)
+     apply (simp add: consistent_medial_coin50)
+     apply (simp add: apply_coin50_updates apply_coin_updates)
+    apply (simp add: consistent_def)
+    apply safe
+    apply (rule_tac x=s in exI)
+    apply (simp add: posterior_def Let_def)
+    apply (simp add: medial_coin50 consistent_medial_coin50)
+    apply (simp add: apply_coin50_updates)
+    apply (simp add: guard_coin consistent_medial_coin)
+    apply (simp add: coin_def remove_input_constraints_def satisfiable_def)
+    by (simp add: consistent_empty_4)
 qed
 
-lemma merge_transitions: "merge_transitions drinks_before merge_1_2 2 1 1 1 1 coin coin50 (\<lambda>a b c d. Map.empty)
-                (\<lambda>a b c d. Some (merge_1_2_update, mapping)) True = Some drinks_after"
+lemma step_vend_fail: "step merge_1_2_update 1 <R 1 := hd b, R 2 := Num 0> ''vend'' [] = Some (vend_fail, 1, [], <R 1 := hd b, R 2 := Num 0>)"
 proof-
-  have no_direct_subsumption_coin_coin50: "\<not> directly_subsumes drinks_before 1 coin coin50"
-  proof-
-    have subsumption_violation: "(\<exists>i r. apply_guards (Guard coin50) (case_vname (\<lambda>n. input2state i 1 (I n)) (\<lambda>n. r (R n))) \<and>
-           apply_outputs (Outputs coin50) (case_vname (\<lambda>n. input2state i 1 (I n)) (\<lambda>n. r (R n))) \<noteq>
-           apply_outputs (Outputs coin) (case_vname (\<lambda>n. input2state i 1 (I n)) (\<lambda>n. r (R n))))"
-      apply (rule_tac x="[Num 50]" in exI)
-      apply (rule_tac x="<>" in exI)
-      by (simp add: transitions)
-    show ?thesis
-      apply (simp add: directly_subsumes_def)
-      apply (rule_tac x="[(''select'', [Str ''coke''])]" in exI)
-      apply safe
-      apply (rule gets_us_to.step_some)
-        apply (simp add: step_def possible_steps_drinks_before_select)
-       apply (simp add: gets_us_to.base)
-      apply (simp add: subsumes_def)
-      using subsumption_violation
-      by auto
-  qed
-  have no_direct_subsumption_coin50_coin: "\<not> directly_subsumes drinks_before 2 coin50 coin"
-  proof-
-    have subsumption_violation: "(\<exists>i r. apply_guards (Guard coin) (case_vname (\<lambda>n. input2state i 1 (I n)) (\<lambda>n. r (R n))) \<and>
-         apply_outputs (Outputs coin50) (case_vname (\<lambda>n. input2state i 1 (I n)) (\<lambda>n. r (R n))) \<noteq>
-         apply_outputs (Outputs coin) (case_vname (\<lambda>n. input2state i 1 (I n)) (\<lambda>n. r (R n))))"
-      apply (rule_tac x="[Num 50]" in exI)
-      apply (rule_tac x="<>" in exI)
-      by (simp add: transitions)
-    show ?thesis
-      apply (simp add: directly_subsumes_def)
-      apply (rule_tac x="[(''select'', [Str ''coke'']), (''coin'', [Num 50])]" in exI)
-      apply safe
-       apply (rule gets_us_to.step_some)
-        apply (simp add: step_def possible_steps_drinks_before_select)
-       apply (rule gets_us_to.step_some)
-        apply (simp add: step_def possible_steps_drinks_before_coin_50)
-       apply (simp add: gets_us_to.base)
-      apply (simp add: subsumes_def)
-      using subsumption_violation
-      by auto
-  qed
-  have easy_merge_none: "easy_merge drinks_before merge_1_2 2 1 1 1 1 coin coin50 (\<lambda>a b c d. Map.empty) = None"
-    by (simp add: easy_merge_def no_direct_subsumption_coin_coin50 no_direct_subsumption_coin50_coin)
-  have easy_merge_some: "easy_merge merge_1_2_update merge_1_2_update 1 1 1 1 1 coin coin50 (\<lambda>a b c d. Map.empty) = Some drinks_after"
-  proof-
-    have coin_directly_subsumes_coin50: "directly_subsumes merge_1_2_update 1 coin coin50"
-    proof-
-      show ?thesis
-        apply (simp add: directly_subsumes_def)
-        sorry
-    qed
-    have no_direct_subsumption_coin50_coin: "\<not> directly_subsumes merge_1_2_update 1 coin50 coin"
-    proof-
-      have subsumption_violation:  "\<not>(\<forall>i r. apply_guards (Guard coin) (\<lambda>x. case x of I n \<Rightarrow> input2state i 1 (I n) | R n \<Rightarrow> r (R n)) \<longrightarrow>
-           apply_outputs (Outputs coin) (\<lambda>x. case x of I n \<Rightarrow> input2state i 1 (I n) | R n \<Rightarrow> r (R n)) =
-           apply_outputs (Outputs coin50) (\<lambda>x. case x of I n \<Rightarrow> input2state i 1 (I n) | R n \<Rightarrow> r (R n)))"
-        apply simp
-        apply (rule_tac x="[Num 50]" in exI)
-        apply (rule_tac x="<>" in exI)
-        by (simp add: transitions)
-      show ?thesis
-        apply (simp add: directly_subsumes_def)
-        apply (rule_tac x="[(''select'', [Str ''coke''])]" in exI)
-        apply safe
-         apply (rule gets_us_to.step_some)
-          apply (simp add: step_def possible_steps_merge_1_2_update_select)
-         apply (simp add: gets_us_to.base)
-        by (simp add: subsumes_def subsumption_violation)
-    qed
-    have set_filter: "Set.filter (\<lambda>x. x \<noteq> ((1, 1), coin50)) (fset merge_1_2_update) =
-          {((0, 1), select_update), ((1, 1), coin), ((1, 1), vend_fail), ((1, 3), vend_success)}"
-      apply (simp add: merge_1_2_update_def Set.filter_def)
-      apply safe
-      by (simp_all add: transitions)
-    have abs_fset: "Abs_fset {((0, 1), select_update), ((1, 1), coin), ((1, 1), vend_fail), ((1, 3), vend_success)} =
-                            {|((0, 1), select_update), ((1, 1), coin), ((1, 1), vend_fail), ((1, 3), vend_success)|}"
-      by (metis finsert.rep_eq fset_inverse fset_simps(1))
-    show ?thesis
-      apply (simp add: easy_merge_def coin_directly_subsumes_coin50 no_direct_subsumption_coin50_coin)
-      apply (simp add: replace_transition_def ffilter_def set_filter abs_fset)
-      apply (simp add: drinks_after_def)
-      by auto
-  qed
+  have set_filter: "(Set.filter
+          (\<lambda>((origin, dest), t).
+              origin = 1 \<and>
+              Label t = ''vend'' \<and>
+              Arity t = 0 \<and> apply_guards (Guard t) (case_vname Map.empty (\<lambda>n. if n = 2 then Some (Num 0) else <R 1 := hd b> (R n))))
+          (fset merge_1_2_update)) = {((1, 1), vend_fail)}"
+    apply (simp add: merge_1_2_update_def Set.filter_def)
+    apply safe
+    by (simp_all add: transitions)
   show ?thesis
-    apply (simp add: merge_transitions_def easy_merge_none mapping_def)
-    by (simp add: simulation easy_merge_some)
+    apply (simp add: step_def possible_steps_def ffilter_def set_filter)
+    apply (simp add: step_def possible_steps_def ffilter_def set_filter)
+    by (simp add: vend_fail_def)
 qed
+
+lemma posterior_vend_fail: "posterior \<lbrakk>V (R 1) \<mapsto> cexp.Bc True, V (R 2) \<mapsto> cexp.Eq (Num 0)\<rbrakk> vend_fail =
+       \<lbrakk>V (R 1) \<mapsto> cexp.Bc True, V (R 2) \<mapsto> cexp.Eq (Num 0)\<rbrakk>"
+proof-
+  have medial: "medial \<lbrakk>V (R 1) \<mapsto> cexp.Bc True, V (R 2) \<mapsto> cexp.Eq (Num 0)\<rbrakk> (Guard vend_fail) =
+        \<lbrakk>V (R 1) \<mapsto> cexp.Bc True, V (R 2) \<mapsto> And (cexp.Eq (Num 0)) (cexp.Lt (Num 100))\<rbrakk>"
+    apply (rule ext)
+    by (simp add: vend_fail_def)
+  have consistent: "consistent \<lbrakk>V (R 1) \<mapsto> cexp.Bc True, V (R 2) \<mapsto> And (cexp.Eq (Num 0)) (cexp.Lt (Num 100))\<rbrakk>"
+    apply (simp add: consistent_def)
+    apply (rule_tac x="<R 1 := Num 5, R 2 := Num 0>" in exI)
+    apply clarify
+    by (simp add: consistent_empty_4)
+  show ?thesis
+    unfolding posterior_def Let_def
+    apply (simp add: medial consistent remove_input_constraints_def)
+    apply (rule ext)
+    by (simp add: vend_fail_def)
+qed
+
+lemma merge_1_2_step_0_invalid: "\<not> (aa = ''select'' \<and> length b = 1) \<Longrightarrow> nondeterministic_step merge_1_2 0 Map.empty aa b = None"
+proof-
+  assume premise: "\<not> (aa = ''select'' \<and> length b = 1)"
+  have set_filter: "Set.filter
+           (\<lambda>((origin, dest), t).
+               origin = 0 \<and> Label t = aa \<and> length b = Arity t \<and> apply_guards (Guard t) (case_vname (\<lambda>n. input2state b 1 (I n)) Map.empty))
+           (fset merge_1_2) = {}"
+    using premise
+    apply (simp add: merge_1_2_def Set.filter_def)
+    apply safe
+    by (simp_all add: transitions)
+  show ?thesis
+    by (simp add: nondeterministic_step_def possible_steps_def ffilter_def set_filter)
+qed
+
+lemma nondeterministic_step_merge_1_2_1_invalid: "aa \<noteq> ''coin'' \<Longrightarrow> nondeterministic_step merge_1_2 1 <R 1 := d> aa b = None"
+proof-
+  assume premise: "aa \<noteq> ''coin''"
+  have set_filter: "Set.filter
+           (\<lambda>((origin, dest), t).
+               origin = 1 \<and>
+               Label t = aa \<and>
+               length b = Arity t \<and> apply_guards (Guard t) (case_vname (\<lambda>n. input2state b 1 (I n)) (\<lambda>n. if n = 1 then Some d else None)))
+           (fset merge_1_2) = {}"
+    using premise
+    apply (simp add: Set.filter_def merge_1_2_def)
+    apply safe
+    by (simp_all add: transitions)
+  show ?thesis
+    by (simp add: nondeterministic_step_def possible_steps_def ffilter_def set_filter)
+qed
+
+lemma nondeterministic_step_merge_1_2_1_invalid_coin: "aa = ''coin'' \<Longrightarrow> length b \<noteq> 1 \<Longrightarrow> nondeterministic_step merge_1_2 1 <R 1 := d> aa b = None"
+proof-
+  assume premise1: "aa = ''coin''"
+  assume premise2: "length b \<noteq> 1"
+  have set_filter: "Set.filter
+           (\<lambda>((origin, dest), t).
+               origin = 1 \<and>
+               Label t = aa \<and>
+               length b = Arity t \<and> apply_guards (Guard t) (case_vname (\<lambda>n. input2state b 1 (I n)) (\<lambda>n. if n = 1 then Some d else None)))
+           (fset merge_1_2) = {}"
+    using premise1 premise2
+    apply (simp add: merge_1_2_def Set.filter_def)
+    apply safe
+    by (simp_all add: transitions)
+  show ?thesis
+    by (simp add: nondeterministic_step_def possible_steps_def ffilter_def set_filter)
+qed
+
+lemma nondeterministic_step_merge_1_2_1_silly_coin: "length b = 1 \<Longrightarrow> b \<noteq> [Num 50] \<Longrightarrow> nondeterministic_step merge_1_2 1 <R 1 := d> ''coin'' b = Some (coin, 1, [], <R 1 := d>)"
+proof-
+  assume premise1: "length b = 1"
+  assume premise2: "b \<noteq> [Num 50]"
+  have set_filter: "Set.filter
+            (\<lambda>((origin, dest), t).
+                origin = 1 \<and>
+                Label t = ''coin'' \<and>
+                length b = Arity t \<and> apply_guards (Guard t) (case_vname (\<lambda>n. input2state b 1 (I n)) (\<lambda>n. if n = 1 then Some d else None)))
+            (fset merge_1_2) = {((1, 1), coin)}"
+    using premise1 premise2
+    apply (simp add: Set.filter_def merge_1_2_def)
+    apply safe
+           apply (simp_all add: transitions hd_input2state)
+    by (metis One_nat_def length_0_conv length_Suc_conv list.sel(1))
+  show ?thesis
+    apply (simp add: nondeterministic_step_def possible_steps_def ffilter_def set_filter)
+    apply (simp add: set_filter)
+    apply (simp add: transitions)
+    apply (rule ext)
+    by simp
+qed
+
+lemma easy_merge_some: "easy_merge drinks_before merge_1_2_update 2 1 1 1 1 coin coin50 (\<lambda>a b c d. Map.empty) = Some drinks_after"
+  apply (simp add: easy_merge_def)
+  oops
 
 lemma score_2: "sorted_list_of_fset (score drinks_after naive_score) = [(0, 0, 1), (0, 0, 3), (0, 1, 3)]"
 proof-
@@ -816,7 +931,445 @@ proof-
     by (simp add: sorted_list_of_fset_def)
 qed
 
-lemma "infer drinks_before naive_score (\<lambda>a b c d e. None) (\<lambda>a b c d. Some (merge_1_2_update, mapping)) = drinks_after"
+lemma step_drinks_before_select: "length ba = 1 \<Longrightarrow> step drinks_before 0 Map.empty ''select'' ba = Some (select, 1, [], <R 1 := hd ba>)"
+proof-
+  assume premise: "length ba = 1"
+  show ?thesis
+     apply (simp add: premise step_def possible_steps_drinks_before_select)
+    apply (simp add: select_def)
+    apply (rule ext)
+    by (simp add: hd_input2state premise)
+qed
+
+lemma no_direct_subsumption_coin_coin50: "\<not> directly_subsumes drinks_before merge_1_2 1 coin coin50"
+proof-
+  have subsumption_violation: "(\<exists>i r. satisfies_context r \<lbrakk>V (R 1) \<mapsto> cexp.Bc True\<rbrakk> \<and>
+           apply_guards (Guard coin50) (case_vname (\<lambda>n. input2state i 1 (I n)) (\<lambda>n. r (R n))) \<and>
+           apply_outputs (Outputs coin50) (case_vname (\<lambda>n. input2state i 1 (I n)) (\<lambda>n. r (R n))) \<noteq>
+           apply_outputs (Outputs coin) (case_vname (\<lambda>n. input2state i 1 (I n)) (\<lambda>n. r (R n))))"
+    apply (rule_tac x="[Num 50]" in exI)
+    apply (rule_tac x="<R 1 := Str ''coke''>" in exI)
+    apply standard
+     defer
+    apply (simp add: coin50_def coin_def)
+     apply (simp add: satisfies_context_def consistent_def datastate2context_def)
+     apply (rule_tac x="<R 1 := Str ''coke''>" in exI)
+     apply clarify
+     apply simp
+     apply (case_tac r)
+        apply simp
+       apply simp
+       apply (case_tac x2)
+    by auto
+  show ?thesis
+    apply (simp add: directly_subsumes_def)
+    apply (rule_tac x="[(''select'', [Str ''coke''])]" in exI)
+    apply standard
+     apply (simp add: accepts_trace_def)
+     apply (rule accepts.step)
+      apply (simp add: step_drinks_before_select)
+     apply (rule accepts.base)
+    apply standard
+     apply (rule gets_us_to.step_some)
+      apply (simp add: step_def possible_steps_drinks_before_select)
+     apply (simp add: gets_us_to.base)
+    apply (simp add: anterior_context_def step_def possible_steps_merge_1_2_select select_posterior)
+    by (simp add: subsumes_def subsumption_violation)
+qed
+
+lemma possible_steps_merge_1_2_coin50: "possible_steps merge_1_2 1 r ''coin'' [Num 50] = {|(1, coin), (1, coin50)|}"
+proof-
+  have set_filter: "Set.filter
+       (\<lambda>((origin, dest), t).
+           origin = 1 \<and>
+           Label t = ''coin'' \<and> Suc 0 = Arity t \<and> apply_guards (Guard t) (case_vname (\<lambda>n. input2state [Num 50] 1 (I n)) (\<lambda>n. r (R n))))
+       (fset merge_1_2) = {((1, 1), coin), ((1, 1), coin50)}"
+    apply (simp add: Set.filter_def merge_1_2_def)
+    apply safe
+    by (simp_all add: transitions)
+  have abs_fset: "Abs_fset {((1, 1), coin), ((1, 1), coin50)} = {|((1, 1), coin), ((1, 1), coin50)|}"
+    by (metis finsert.rep_eq fset_inverse fset_simps(1))
+  show ?thesis
+    by (simp add: possible_steps_def ffilter_def set_filter abs_fset)
+qed
+
+lemma step_drinks_before_coin_50: "step drinks_before 1 <R 1 := d> ''coin'' [Num 50] = Some (coin50, 2, [Num 50], <R 1 := d, R 2 := Num 50>)"
+proof-
+  have set_filter: "Set.filter
+          (\<lambda>((origin, dest), t).
+              origin = 1 \<and>
+              Label t = ''coin'' \<and>
+              Suc 0 = Arity t \<and>
+              apply_guards (Guard t)
+               (case_vname (\<lambda>n. if n = 1 then Some (Num 50) else input2state [] (1 + 1) (I n)) (\<lambda>n. if n = 1 then Some d else None)))
+          (fset drinks_before) = {((1, 2), coin50)}"
+    apply (simp add: Set.filter_def drinks_before_def)
+    apply safe
+    by (simp_all add: transitions)
+  show ?thesis
+    apply (simp add: step_def possible_steps_def ffilter_def set_filter)
+    apply (simp add: set_filter)
+    apply (simp add: transitions)
+    apply (rule ext)
+    by simp
+qed
+
+lemma no_direct_subsumption_coin50_coin: "\<not> directly_subsumes drinks_before merge_1_2 2 coin50 coin"
+proof-
+  have subsumption_violation: "(\<exists>i r. satisfies_context r \<lbrakk>V (R 1) \<mapsto> cexp.Bc True\<rbrakk> \<and>
+           apply_guards (Guard coin) (case_vname (\<lambda>n. input2state i 1 (I n)) (\<lambda>n. r (R n))) \<and>
+           apply_outputs (Outputs coin) (case_vname (\<lambda>n. input2state i 1 (I n)) (\<lambda>n. r (R n))) \<noteq>
+           apply_outputs (Outputs coin50) (case_vname (\<lambda>n. input2state i 1 (I n)) (\<lambda>n. r (R n))))"
+apply (rule_tac x="[Num 50]" in exI)
+    apply (rule_tac x="<R 1 := Str ''coke''>" in exI)
+    apply standard
+     defer
+    apply (simp add: coin50_def coin_def)
+     apply (simp add: satisfies_context_def consistent_def datastate2context_def)
+     apply (rule_tac x="<R 1 := Str ''coke''>" in exI)
+     apply clarify
+     apply simp
+     apply (case_tac r)
+        apply simp
+       apply simp
+       apply (case_tac x2)
+    by auto
+  show ?thesis
+    apply (simp add: directly_subsumes_def)
+    apply (rule_tac x="[(''select'', [Str ''coke'']), (''coin'', [Num 50])]" in exI)
+    apply standard
+     apply (simp add: accepts_trace_def)
+     apply (rule accepts.step)
+      apply (simp add: step_drinks_before_select)
+     apply (rule accepts.step)
+      apply (simp add: step_drinks_before_coin_50)
+    apply (rule accepts.base)
+    apply standard
+     apply (rule gets_us_to.step_some)
+      apply (simp add: step_def possible_steps_drinks_before_select)
+     apply (rule gets_us_to.step_some)
+      apply (simp add: step_def possible_steps_drinks_before_coin_50)
+     apply (simp add: gets_us_to.base)
+    apply (simp add: anterior_context_def step_def possible_steps_merge_1_2_select select_posterior)
+    apply (simp add: possible_steps_merge_1_2_coin50 fis_singleton_def is_singleton_def)
+    apply standard
+     apply (simp add: transitions)
+    by (simp add: subsumes_def subsumption_violation)
+qed
+
+lemma easy_merge_none:  "easy_merge drinks_before merge_1_2 2 1 1 1 1 coin coin50 (\<lambda>a b c d. Map.empty) = None"
+  by (simp add: easy_merge_def no_direct_subsumption_coin_coin50 no_direct_subsumption_coin50_coin)
+
+lemma regsimp1: "(\<lambda>a. if a = R 1 then Some d else None) = <R 1 := d>"
+  by auto
+
+lemma contextsimp1: "(\<lambda>a. if a = V (R 2) then cexp.Eq (Num 0) else if a = V (R 1) then cexp.Bc True else \<lbrakk>\<rbrakk> a) = 
+                     \<lbrakk>V (R 1) \<mapsto> cexp.Bc True, V (R 2) \<mapsto> cexp.Eq (Num 0)\<rbrakk>"
+  by auto
+
+lemma regsimp2: "(\<lambda>a. if a = R 2 then Some (Num n) else if a = R 1 then Some d else None) = <R 1 := d, R 2 := Num n>"
+  by auto
+
+lemma invalid_r2_vend: "\<nexists>n. ra (R 2) = Some (Num n) \<Longrightarrow> step drinks_before 2 ra ''vend'' [] = None"
+proof-
+  assume premise: "\<nexists>n. ra (R 2) = Some (Num n)"
+  have set_filter: "(Set.filter
+         (\<lambda>((origin, dest), t). origin = 2 \<and> Label t = ''vend'' \<and> Arity t = 0 \<and> apply_guards (Guard t) (case_vname Map.empty (\<lambda>n. ra (R n))))
+         (fset drinks_before)) = {}"
+    using premise
+    apply (simp add: Set.filter_def drinks_before_def)
+    apply safe
+      apply (simp add: transitions)
+    apply (simp add: transitions)
+     apply (metis MaybeBoolInt.elims option.simps(3))
+    apply (simp add: transitions)
+    apply (case_tac "MaybeBoolInt (\<lambda>x y. y < x) (Some (Num 100)) (ra (R 2))")
+     apply simp
+    apply simp
+    by (metis MaybeBoolInt.elims option.simps(3))
+  show ?thesis
+    by (simp add: step_def possible_steps_def ffilter_def set_filter)
+qed
+
+lemma step_drinks_before_vend_fail: "ra (R 2) = Some (Num x1) \<Longrightarrow> x1 < 100 \<Longrightarrow> step drinks_before 2 ra ''vend'' [] = Some (vend_fail, 2, [], ra)"
+proof-
+  assume premise1: "ra (R 2) = Some (Num x1)"
+  assume premise2: "x1 < 100"
+  have set_filter: "Set.filter
+          (\<lambda>((origin, dest), t).
+              origin = 2 \<and> Label t = ''vend'' \<and> Arity t = 0 \<and> apply_guards (Guard t) (case_vname Map.empty (\<lambda>n. ra (R n))))
+          (fset drinks_before) = {((2, 2), vend_fail)}"
+    using premise1 premise2
+    apply (simp add: Set.filter_def drinks_before_def)
+    apply safe
+    by (simp_all add: transitions)
+  show ?thesis
+    apply (simp add: step_def possible_steps_def ffilter_def set_filter)
+    apply (simp add: set_filter)
+    by (simp add: transitions)
+qed
+
+lemma step_drinks_before_3_none: "step drinks_before 3 r' a b = None"
+proof-
+  have set_filter: "Set.filter
+         (\<lambda>((origin, dest), t).
+             origin = 3 \<and> Label t = a \<and> length b = Arity t \<and> apply_guards (Guard t) (case_vname (\<lambda>n. input2state b 1 (I n)) (\<lambda>n. r' (R n))))
+         (fset drinks_before) = {}"
+    by (simp add: Set.filter_def drinks_before_def)
+  show ?thesis
+    by (simp add: step_def possible_steps_def ffilter_def set_filter)
+qed
+
+lemma no_route_from_3_to_anywhere: "s \<noteq> 3 \<Longrightarrow> \<not>gets_us_to s drinks_before 3 r' p"
+  apply safe
+  apply (rule gets_us_to.cases)
+     apply simp
+    apply simp
+   apply (simp add: step_drinks_before_3_none)
+  by simp
+
+lemma no_route_from_2_to_1: "\<forall>r. \<not>gets_us_to 1 drinks_before 2 r p"
+proof(induct p)
+  case Nil
+  then show ?case
+    by (simp add: no_further_steps)
+next
+  case (Cons a p)
+  then show ?case
+    apply clarify
+    apply (rule gets_us_to.cases)
+       apply simp
+      apply simp
+     defer
+     apply simp
+    apply clarify
+    apply simp
+    apply (case_tac "aa = ''coin'' \<and> length b = 1")
+     apply (simp add: step_def possible_steps_drinks_before_coin)
+    apply (case_tac "aa = ''vend'' \<and> b = []")
+    defer
+    apply (simp add: nondeterministic_step_drinks_before_invalid_step_2 nondeterministic_step_none)
+     apply clarify
+     apply simp
+     apply (case_tac "ra (R 2)")
+      apply (simp add: invalid_r2_vend)
+     apply (case_tac aa)
+      defer
+     apply (simp add: invalid_r2_vend)
+    apply clarify
+    apply simp
+    apply (case_tac "x1 < 100")
+     apply (simp add: step_drinks_before_vend_fail)
+    apply (simp add: step_def drinks_before_vend_success)
+    apply (simp add: vend_success_def)
+    apply clarify
+    by (simp add: no_route_from_3_to_anywhere)
+qed
+
+lemma drinks_before_1_step_invalid: "(aa, ba) \<noteq> (''coin'', [Num 50]) \<Longrightarrow> step drinks_before 1 r aa ba = None"
+proof-
+  assume premise: "(aa, ba) \<noteq> (''coin'', [Num 50])"
+  have set_filter: "Set.filter
+         (\<lambda>((origin, dest), t).
+             origin = 1 \<and>
+             Label t = aa \<and> length ba = Arity t \<and> apply_guards (Guard t) (case_vname (\<lambda>n. input2state ba 1 (I n)) (\<lambda>n. r (R n))))
+         (fset drinks_before) = {}"
+    using premise
+    apply (simp add: Set.filter_def drinks_before_def)
+    apply safe
+     apply (simp_all add: transitions)
+    by (metis One_nat_def hd_input2state le_numeral_extra(4) length_0_conv length_Suc_conv list.sel(1) option.inject)
+  show ?thesis
+    by (simp add: step_def possible_steps_def ffilter_def set_filter)
+qed
+
+lemma stop_at_1: "step drinks_before 1 <R 1 := d> aa ba = Some (uw, s', ux, r') \<Longrightarrow> \<not>gets_us_to 1 drinks_before 1 <R 1 := d> ((aa, ba) # p)"
+  apply safe
+  apply (rule gets_us_to.cases)
+     apply simp
+    apply simp
+  apply (case_tac "(aa, ba) = (''coin'', [Num 50])")
+   apply (simp add: step_drinks_before_coin_50)
+    apply clarify
+    apply simp
+    apply clarify
+    apply simp
+   apply (simp add: step_drinks_before_coin_50)
+    apply clarify
+    apply (simp add: no_route_from_2_to_1)
+   apply (simp add: drinks_before_1_step_invalid)
+   apply clarify
+  by simp
+
+lemma drinks_before_1_must_be_coin_50: "fis_singleton (possible_steps drinks_before 1 <R 1 := d> aa ba) \<Longrightarrow> (aa = ''coin'' \<and> ba = [Num 50])"
+proof-
+  assume premise: "fis_singleton (possible_steps drinks_before 1 <R 1 := d> aa ba)"
+  have set_filter: "\<not> (aa = ''coin'' \<and> ba = [Num 50]) \<Longrightarrow> Set.filter
+         (\<lambda>((origin, dest), t).
+             origin = 1 \<and>
+             Label t = aa \<and>
+             length ba = Arity t \<and> apply_guards (Guard t) (case_vname (\<lambda>n. input2state ba 1 (I n)) (\<lambda>n. if n = 1 then Some d else None)))
+         (fset drinks_before) = {}"
+    apply (simp add: Set.filter_def drinks_before_def)
+    apply (simp add: transitions)
+    by (metis One_nat_def hd_input2state le_numeral_extra(4) length_0_conv length_Suc_conv list.sel(1) option.inject)
+  show ?thesis
+    using premise
+    apply (case_tac "aa = ''coin'' \<and> ba = [Num 50]")
+     apply simp
+    by (simp add: possible_steps_def ffilter_def set_filter)
+qed
+
+lemma gets_us_to_aux: "gets_us_to 1 drinks_before 1 <R 1 := d> p \<Longrightarrow> accepts drinks_before 1 <R 1 := d> p \<Longrightarrow>
+          posterior_sequence \<lbrakk>V (R 1) \<mapsto> cexp.Bc True, V (R 2) \<mapsto> cexp.Eq (Num 0)\<rbrakk> merge_1_2_update 1 <R 1 := d, R 2 := Num 0> p =
+          \<lbrakk>V (R 1) \<mapsto> cexp.Bc True, V (R 2) \<mapsto> cexp.Eq (Num 0)\<rbrakk>"
+proof (induct p)
+  case Nil
+  then show ?case
+  by simp
+next
+  case (Cons a p)
+  then show ?case
+    apply (case_tac a)
+    apply clarify
+    apply (simp del: posterior_sequence.simps)
+    apply (simp only: regsimp1 regsimp2 contextsimp1) \<comment> \<open>This makes it print nicely again\<close>
+    apply (rule gets_us_to.cases)
+       apply simp
+      apply simp
+     apply simp
+    apply clarify
+     apply (simp del: posterior_sequence.simps)
+     apply (simp add: stop_at_1)
+    apply clarify
+    apply simp
+    apply (case_tac "step merge_1_2_update 1 <R 1 := d, R 2 := Num 0> aa ba")
+     apply simp
+    apply simp
+    apply clarify
+    by (simp add: no_step_none)
+qed
+
+lemma accepts_trace_anterior: "accepts_trace drinks_before p \<Longrightarrow> gets_us_to 1 drinks_before 0 Map.empty p \<Longrightarrow> anterior_context merge_1_2_update p = \<lbrakk>V (R 1) \<mapsto> Bc True, V (R 2) \<mapsto> Eq (Num 0)\<rbrakk>"
+proof(induct p)
+  case Nil
+  then show ?case
+    apply simp
+    apply (rule gets_us_to.cases)
+    by auto
+next
+  have select_update_updates: "\<forall>ba. length ba = 1 \<longrightarrow> (EFSM.apply_updates (Updates select_update) (case_vname (\<lambda>n. input2state ba 1 (I n)) Map.empty) Map.empty) =
+        <R 1 := hd ba, R 2 := Num 0>"
+    apply clarify
+    apply (rule ext)
+    by (simp add: transitions hd_input2state)
+  case (Cons a p)
+  then show ?case
+    apply (case_tac a)
+    apply (case_tac "aa = ''select'' \<and> length b = 1")
+    defer
+     apply clarify
+     apply (rule gets_us_to.cases)
+        apply simp
+       apply simp
+    using drinks_before_step_0_invalid nondeterministic_step_none
+      apply auto[1]
+     apply simp
+
+    apply (rule gets_us_to.cases)
+       apply simp
+      apply simp
+     defer
+     apply clarify
+     apply (simp add: step_def possible_steps_drinks_before_select)
+
+    apply clarify
+    apply (simp add: step_drinks_before_select)
+    apply clarify
+    apply (simp add: anterior_context_def step_def possible_steps_merge_1_2_update_select)
+    apply (simp add: accepts_trace_def)
+    apply (rule accepts.cases)
+      apply simp
+     apply simp
+    apply simp
+    apply clarify
+    apply (simp add: step_drinks_before_select)
+    apply clarify
+    apply (simp add: select_update_posterior select_update_updates)
+    by (simp add: gets_us_to_aux)
+qed
+
+lemma coin_directly_subsumes_coin50: "directly_subsumes drinks_before merge_1_2_update 1 coin coin50"
+  apply (simp add: directly_subsumes_def)
+  apply clarify
+  by (simp add: accepts_trace_anterior coin_subsumes_coin50)
+
+lemma step_merge_1_2_update_select: "step merge_1_2_update 0 Map.empty ''select'' [d] = Some (select_update, 1, [], <R 1 := d, R 2 := Num 0>)"
+  apply (simp add: step_def possible_steps_merge_1_2_update_select)
+  apply (simp add: transitions)
+  apply (rule ext)
+  by simp
+
+lemma step_merge_1_2_update_coin_50: "step merge_1_2_update 1 <R 1 := Str ''coke'', R 2 := Num 0> ''coin'' [Num 50] = None"
+  apply (simp add: step_def merge_1_2_update_possible_steps_coin_50 fis_singleton_def is_singleton_def)
+  by (simp add: transitions)
+
+lemma coin50_doesnt_subsume_coin: "\<not> subsumes \<lbrakk>V (R 1) \<mapsto> cexp.Bc True, V (R 2) \<mapsto> cexp.Eq (Num 0)\<rbrakk> coin50 coin"
+proof-
+  have subsumption_violation: "(\<exists>r i. cval (medial \<lbrakk>V (R 1) \<mapsto> cexp.Bc True, V (R 2) \<mapsto> cexp.Eq (Num 0)\<rbrakk> (Guard coin) r) i = Some True \<and>
+           cval (medial \<lbrakk>V (R 1) \<mapsto> cexp.Bc True, V (R 2) \<mapsto> cexp.Eq (Num 0)\<rbrakk> (Guard coin50) r) i \<noteq> Some True)"
+    apply (simp add: transitions)
+    by auto
+  show ?thesis
+    by (simp add: subsumes_def subsumption_violation)
+qed
+
+lemma coin50_doesnt_directly_subsume_coin: "\<not> directly_subsumes drinks_before merge_1_2_update 2 coin50 coin"
+proof-
+  show ?thesis
+    apply (simp add: directly_subsumes_def)
+    apply (rule_tac x="[(''select'', [Str ''coke'']), (''coin'', [Num 50])]" in exI)
+    apply standard
+     apply (simp add: accepts_trace_def)
+     apply (rule accepts.step)
+      apply (simp add: step_drinks_before_select)
+     apply (rule accepts.step)
+      apply (simp add: step_drinks_before_coin_50)
+     apply (rule accepts.base)
+    apply standard
+    apply (rule gets_us_to.step_some)
+      apply (simp add: step_drinks_before_select)
+    apply (rule gets_us_to.step_some)
+      apply (simp add: step_drinks_before_coin_50)
+     apply (simp add: gets_us_to.base)
+    apply (simp add: anterior_context_def)
+    apply (simp add: step_merge_1_2_update_select step_merge_1_2_update_coin_50)
+    by (simp add: select_update_posterior coin50_doesnt_subsume_coin)
+qed
+
+lemma easy_merge_some: "easy_merge drinks_before merge_1_2_update 2 1 (update_mapping 1) (update_mapping 1) (update_mapping 1) coin coin50 (\<lambda>a b c d. Map.empty) =
+    Some drinks_after"
+proof-
+  have set_filter: "Set.filter (\<lambda>x. x \<noteq> ((1, 1), coin50)) (fset merge_1_2_update) = {((0, 1), select_update), ((1, 1), coin), ((1, 1), vend_fail), ((1, 3), vend_success)}"
+    apply (simp add: merge_1_2_update_def Set.filter_def)
+    apply safe
+    by (simp_all add: transitions)
+  have abs_fset: "Abs_fset {((0, 1), select_update), ((1, 1), coin), ((1, 1), vend_fail), ((1, 3), vend_success)} =
+                          {|((0, 1), select_update), ((1, 1), coin), ((1, 1), vend_fail), ((1, 3), vend_success)|}"
+    by (metis finsert.rep_eq fset_inverse fset_simps(1))
+  show ?thesis
+  apply (simp add: easy_merge_def coin_directly_subsumes_coin50 coin50_doesnt_directly_subsume_coin)
+    apply (simp add: replace_transition_def update_mapping_def ffilter_def set_filter abs_fset)
+    using drinks_after_def
+    by auto
+qed
+
+lemma merge_transitions: "merge_transitions drinks_before merge_1_2 2 1 1 1 1 coin coin50 (\<lambda>a b c d. Map.empty)
+                (\<lambda>a b c d e. Some (merge_1_2_update, update_mapping, update_before)) True = Some drinks_after"
+  apply (simp add: merge_transitions_def easy_merge_none)
+  by (simp add: simulation easy_merge_some)
+
+lemma "infer drinks_before naive_score (\<lambda>a b c d e. None) (\<lambda>a b c d e. Some (merge_1_2_update, update_mapping, update_before)) = drinks_after"
 proof-
   have nondeterminism_merge_1_2: "nondeterminism merge_1_2"
     by (simp add: nondeterminism_def nondeterministic_pairs)
@@ -824,8 +1377,8 @@ proof-
     apply (simp add: score sorted_list_of_fset_def Let_def)
     apply (simp add: merge_1_2 nondeterministic_pairs)
     apply (simp add: coin_doesnt_exit_1_drinks_before coin50_exits_1_drinks_before)
-    apply (simp add: nondeterminism_merge_1_2 merge_transitions)
+    apply (simp add: nondeterminism_merge_1_2)
+    apply (simp add: merge_transitions)
     by (simp add: score_2)
 qed
-
 end
